finish proof for sc and tso example.

LeanCats/Examples.lean
@@ -1,20 +1,20 @@
 import LeanCats.Data
 import LeanCats.Relations
+import LeanCats.Theoriems
 
 open CatRel
 open Data
 
 namespace SC
 variable (evts : Data.Events)
-variable (co : Rel Data.Event Data.Event)
+variable (coConst : IsStrictTotalOrder Event (preCo evts))
 
-
-@[simp] def X : Data.CandidateExecution :=
+@[simp] def X [IsStrictTotalOrder Event (preCo evts)] : Data.CandidateExecution :=
   {
     evts := evts
-    po := Data.Rel.po
-    fr := Data.Rel.fr co
-    rf := Data.Rel.rf
+    po := CatRel.po evts
+    fr := CatRel.fr evts
+    rf := CatRel.rf.wellformed evts
     IW := evts.IW
   }
 
@@ -25,26 +25,26 @@ and the operations of each individual thread appear in this sequence in the orde
 specified by its program.-/
 
 -- We define the communication between threads as com:
-@[simp] def com := union (X evts co).rf (union co (X evts co).fr)
+@[simp] def com := (X evts).rf ∪ ((co.wellformed evts) ∪ (X evts).fr)
 
 -- Then we union it with the po, the SC ensures that every instructions are executed in program order.
-@[simp] def sc := union (com evts co) ((X evts co).po)
+@[simp] def sc := (com evts coConst) ∪ ((X evts).po)
 
 -- We should avoid the cyclic, because the fr in a ghb will leads a overwritten that violates the program order.
-@[simp] def assert := Acyclic (sc evts co)
+@[simp] def assert := Acyclic (sc evts coConst)
 
 end SC
 
 namespace TSO01
 variable (evts : Events)
-variable (co : Rel Event Event)
+variable (coConst : IsStrictTotalOrder Event (preCo evts))
 
 @[simp] def X : CandidateExecution :=
   {
     evts := evts
-    po := Data.Rel.po
-    fr := Data.Rel.fr co
-    rf := Data.Rel.rf
+    po := CatRel.po evts
+    fr := CatRel.fr evts
+    rf := CatRel.rf.wellformed evts
     IW := evts.IW
   }
 
@@ -52,15 +52,15 @@ variable (co : Rel Event Event)
 A TSO is a memory model that allows the write read out of order in the same thread (write buffer).-/
 
 -- We define the communication between threads as com as in SC:
-@[simp] def com := union (external ∪ (X evts co).rf) (co ∪ ((X evts co).fr))
+@[simp] def com := (external evts ∩ (X evts coConst).rf) ∪ (co.wellformed evts ∪ ((X evts coConst).fr))
 
 -- Then we minus the internal read from and W*R from the po, because we allow them to be out of order.
-@[simp] def po_tso := (X evts co).po ∩ ((prod W W) ∪ (prod R M))
+@[simp] def po_tso := (X evts coConst).po ∩ ((prod W W) ∪ (prod R M))
 
-@[simp] def ghb := (po_tso evts co) ∪ (com evts co)
+@[simp] def ghb := (po_tso evts coConst) ∪ (com evts coConst)
 
 -- We should avoid the cyclic, because the fr in a ghb will leads a overwritten that violates the program order.
-@[simp] def assert := Acyclic (ghb evts co)
+@[simp] def assert := Acyclic (ghb evts coConst)
 
 end TSO01
 
@@ -69,10 +69,32 @@ end TSO01
 -- In this case, if we find the ghb is acyclic then tso must also be acyclic because sc models more edges.
 
 -- https://leanprover-community.github.io/mathlib4_docs/Mathlib/Order/Defs/Unbundled.html#IsIrrefl
-theorem scvtso (evts : Data.Events) (co : Rel Data.Event Data.Event) : SC.assert evts co → TSO01.assert evts co :=
+theorem scvtso (evts : Data.Events) [coConst : IsStrictTotalOrder Event (preCo evts)] : SC.assert evts coConst → TSO01.assert evts coConst :=
 by
   simp
   intro sc
-
-
-  sorry
+  apply ayclicMono sc
+  intro a b
+  intro tso
+  cases tso with
+  | inl h => {
+    simp at h
+    apply Or.inr
+    obtain ⟨l, r⟩ := h
+    exact l
+  }
+  | inr h => {
+    obtain ⟨l⟩ := h
+    {
+      apply Or.inl
+      apply Or.inl
+      obtain ⟨l, r⟩ := l
+      exact r
+    }
+    {
+      rename_i h
+      apply Or.inl
+      apply Or.inr
+      exact h
+    }
+  }
